change names to equipotent and bijection

data/fintype.lean
@@ -1,17 +1,16 @@
-import equivalent data.fin.misc
-import data.list.distinct
+import equipotent data.fin.misc
 universe u
 
 class fintype (α : Type u) := 
   (size : ℕ)
-  (finitary : equivalent α (fin size))
+  (finitary : equipotent α (fin size))
 
 namespace fintype
 variables {α : Type u}[fintype α]
 @[reducible]
 def enum : α → fin (size α) := (finitary α).map
 @[reducible]
-def index : fin (size α) → α := (finitary α).iso.inv
+def index : fin (size α) → α := (finitary α).has_bijection.inv
 
 
 def elems : list α := list.map (@index α _) (fin.elems (size α))
@@ -25,7 +24,7 @@ theorem mem_elems : ∀ a : α, a ∈ (elems : list α) :=
           apply fin.mem_elems
       },
     simp [enum,index] at H,
-    rw (finitary α).iso.left_inverse_of_inv at H,
+    rw (finitary α).has_bijection.left_inverse_of_inv at H,
     assumption 
   end
 
