equipotent.lean
@@ -1,51 +1,53 @@
-import function.isomorphism
+import function.bijection
 import data.fin.misc
 universes u v
 open function
 
 
-class equivalent (α : Sort u) (β : Sort v) := 
+class equipotent (α : Sort u) (β : Sort v) := 
   (map : α → β)
-  (iso : isomorphism map)
+  (has_bijection : bijection map)
 
-namespace equivalent
+namespace equipotent
 variables {α : Sort u} {β : Sort v}
 
 @[refl]
-instance rfl : equivalent α α := 
+instance rfl : equipotent α α := 
   {
       map := id,
-      iso := isomorphism.of_id
+      has_bijection := bijection.of_id
   }
 
 @[symm]
-instance symm (eqv : equivalent α β) : equivalent β α := 
+instance symm (eqv : equipotent α β) : equipotent β α := 
  {
-     map := eqv.iso.inv,
-     iso := isomorphism.inverse eqv.iso
+     map := eqv.has_bijection.inv,
+     has_bijection := bijection.inverse eqv.has_bijection
  }
 
  universe w
  variable {γ : Sort w}
  @[trans]
- instance trans (eqv₁ : equivalent α β) (eqv₂ : equivalent β γ) : equivalent α γ := 
+ instance trans (eqv₁ : equipotent α β) (eqv₂ : equipotent β γ) : equipotent α γ := 
  {
      map := eqv₂.map ∘ eqv₁.map,
-     iso := isomorphism.comp eqv₁.iso eqv₂.iso
+     has_bijection := bijection.comp eqv₁.has_bijection eqv₂.has_bijection
  }
-end equivalent
 
-def equivalent_map (α : Sort u) (β : Sort v) := { f : α → β // has_isomorphism f }
-def is_equivalent (α : Sort u) (β : Sort v) := ∃ f : α → β, has_isomorphism f
 
-namespace is_equivalent
+end equipotent
+
+
+def is_equipotent (α : Sort u) (β : Sort v) := ∃ f : α → β, has_bijection f
+
+namespace is_equipotent
 variables {α : Sort u}{β : Sort v}
 
 @[refl]
-def rfl : is_equivalent α α := exists.intro id (exists.intro id (and.intro (take x, rfl) (take x, rfl)))
+def rfl : is_equipotent α α := exists.intro id (exists.intro id (and.intro (take x, rfl) (take x, rfl)))
 
 @[symm]
-def symm : is_equivalent α β → is_equivalent β α := 
+def symm : is_equipotent α β → is_equipotent β α := 
   assume Heqv,
   exists.elim Heqv (λ f ex, exists.elim ex (λ g h, exists.intro g (exists.intro f (and.intro h.right h.left))))
 
@@ -53,18 +55,18 @@ universe w
 variable {γ : Sort w}
 
 @[trans]
-def trans : is_equivalent α β → is_equivalent β γ → is_equivalent α γ :=
+def trans : is_equipotent α β → is_equipotent β γ → is_equipotent α γ :=
   begin
   intros Hab Hbc,
-  cases Hab with f f_iso,
-  cases Hbc with g g_iso,
+  cases Hab with f f_has_bijection,
+  cases Hbc with g g_has_bijection,
   apply exists.intro,
-  apply has_isomorphism.trans,
-  exact f_iso,
-  exact g_iso
+  apply has_bijection.trans,
+  exact f_has_bijection,
+  exact g_has_bijection
   end
 
-def is_equivalent_iff_iff {α : Prop} {β : Prop} : (α ↔ β) ↔ is_equivalent α β :=
+def is_equipotent_iff_iff {α : Prop} {β : Prop} : (α ↔ β) ↔ is_equipotent α β :=
   begin
     apply iff.intro,
       {
@@ -83,30 +85,30 @@ def is_equivalent_iff_iff {α : Prop} {β : Prop} : (α ↔ β) ↔ is_equivalen
           assumption, assumption
       }
   end
-end is_equivalent
+end is_equipotent
 
-def is_finitary (α : Sort u) n := is_equivalent α (fin n)
+def is_finitary (α : Sort u) n := is_equipotent α (fin n)
 
 namespace is_finitary
 
 lemma eq_size_of_fin {m n} : is_finitary (fin m) n → m = n :=
-   assume ⟨f, Hiso⟩,
+   assume ⟨f, Hhas_bijection⟩,
    
    if Heq  : m = n then 
      Heq
    else if Hlt : m < n then
-     exists.elim Hiso (take g, assume Hg, 
+     exists.elim Hhas_bijection (take g, assume Hg, 
        have Hinj : injective g, from injective_of_left_inverse Hg.right,
        absurd Hinj (fin.not_injective_of_gt g Hlt)
        )
    else
-     have Hinj : injective f, from has_isomorphism.injective_of_has_isomorphism Hiso,
+     have Hinj : injective f, from has_bijection.injective_of_has_bijection Hhas_bijection,
      have m > n, from lt_of_le_of_ne (le_of_not_gt Hlt) (ne.symm Heq),
      absurd Hinj (fin.not_injective_of_gt f this)
 
 theorem eq_of_size {m n}{α : Sort u} : is_finitary α m → is_finitary α n → m = n :=
   assume Hm Hn,
-  have is_finitary (fin m) n, from is_equivalent.trans (is_equivalent.symm Hm) Hn,
+  have is_finitary (fin m) n, from is_equipotent.trans (is_equipotent.symm Hm) Hn,
   eq_size_of_fin this
 
 end is_finitary
