function/bijection.lean
@@ -1,0 +1,99 @@
+universes u v
+open function
+
+class bijection {α : Sort u} {β : Sort v} (f : α → β) :=
+  (inv : β → α)
+  (left_inverse_of_inv : left_inverse inv f)
+  (right_inverse_of_inv : right_inverse inv f)
+
+namespace bijection
+variables {α : Sort u} {β : Sort v} {f : α → β}
+
+
+instance of_id : bijection (@id α) :=
+  ⟨ id, take a, rfl, take a, rfl⟩ 
+
+instance inverse (iso_f : bijection f) : bijection (inv f) :=
+  ⟨f, right_inverse_of_inv f, left_inverse_of_inv f⟩ 
+
+def injective_of_bijection (iso_f : bijection f) : injective f :=
+  injective_of_left_inverse (left_inverse_of_inv f)
+
+lemma eq_of_inv_of_bijection (iso₁ iso₂: bijection f) : iso₁.inv = iso₂.inv :=
+begin
+  apply funext,
+  intro,
+  apply injective_of_bijection,
+  assumption,
+  rw iso₁.right_inverse_of_inv,
+  rw iso₂.right_inverse_of_inv
+end
+
+lemma bijection_of_iff {a b : Prop} (h : a ↔ b) : bijection (h.mp) :=
+{
+  inv := h.mpr,
+  left_inverse_of_inv := take p, proof_irrel _ _,
+  right_inverse_of_inv := take p, proof_irrel _ _
+}
+
+private def has_right_inverse_of_bijection (iso_f : bijection f) : has_right_inverse f := ⟨ inv f ,  right_inverse_of_inv f⟩ 
+
+def surjective_of_bijection (iso_f : bijection f) : surjective f := 
+  surjective_of_has_right_inverse (has_right_inverse_of_bijection iso_f)
+
+def bijective_of_bijection (iso_f : bijection f) : bijective f := ⟨ injective_of_bijection iso_f , surjective_of_bijection iso_f⟩
+
+universe w
+variables {γ : Sort w} {g : β → γ}
+instance comp (iso_f : bijection f) (iso_g : bijection g) : bijection (g ∘ f) := 
+ ⟨ inv f ∘ inv g, 
+   begin
+     intro a,
+     simp [comp],
+     repeat {rw [left_inverse_of_inv]}
+   end, 
+   begin
+     intro c,
+     simp [comp],
+     rw [right_inverse_of_inv f, right_inverse_of_inv g]
+   end⟩ 
+end bijection
+
+def has_bijection {α : Sort u}{β : Sort v} (f : α → β) := ∃ g : β → α, left_inverse g f ∧ right_inverse g f
+
+namespace has_bijection
+variables {α : Sort u}{β : Sort v} {f : α → β}
+
+def injective_of_has_bijection : has_bijection f → injective f :=
+  λ ex, exists.elim ex (λ g h, injective_of_left_inverse (and.left h))
+def surjective_of_has_bijection : has_bijection f → surjective f :=
+  λ ex, exists.elim ex (λ g h, surjective_of_has_right_inverse (exists.intro g (and.right h)))
+
+def bijective_of_has_bijection : has_bijection f → bijective f := λ h, and.intro (injective_of_has_bijection h) (surjective_of_has_bijection h)
+
+def of_bijection [ins : bijection f] : has_bijection f := exists.intro ins.inv (and.intro ins.left_inverse_of_inv ins.right_inverse_of_inv)
+
+universe w
+variables {γ : Sort w} {g : β → γ}
+
+
+def trans : has_bijection f → has_bijection g → has_bijection (g ∘ f) :=
+begin
+intros fH gH,
+cases fH with f_inv f_inv_h,
+cases gH with g_inv g_inv_h,
+apply (exists.intro (f_inv ∘ g_inv)),
+apply and.intro,
+{
+    intro x,
+    simp [comp],
+    rw [g_inv_h.left, f_inv_h.left]
+},
+{
+    intro x,
+    simp [comp],
+    rw [f_inv_h.right, g_inv_h.right]
+}
+end
+end has_bijection
+
